Begin with exercises

plf/Typechecking.v
@@ -7,3 +7,213 @@ From PLF Require Import Stlc.
 From PLF Require MoreStlc.
 Module STLCTypes.
 Export STLC.
+
+Fixpoint eqb_ty (T1 T2:ty) : bool :=
+  match T1,T2 with
+  | <{ Bool }> , <{ Bool }> =>
+      true
+  | <{ T11->T12 }>, <{ T21->T22 }> =>
+      andb (eqb_ty T11 T21) (eqb_ty T12 T22)
+  | _,_ =>
+      false
+  end.
+  
+Lemma eqb_ty_refl : forall T,
+  eqb_ty T T = true.
+Proof.
+  intros T. induction T; simpl.
+    reflexivity.
+    rewrite IHT1. rewrite IHT2. reflexivity. Qed.
+
+Lemma eqb_ty__eq : forall T1 T2,
+  eqb_ty T1 T2 = true -> T1 = T2.
+Proof with auto.
+  intros T1. induction T1; intros T2 Hbeq; destruct T2; inversion Hbeq.
+  - (* T1=Bool *)
+    reflexivity.
+  - (* T1 = T1_1->T1_2 *)
+    rewrite andb_true_iff in H0. inversion H0 as [Hbeq1 Hbeq2].
+    apply IHT1_1 in Hbeq1. apply IHT1_2 in Hbeq2. subst... Qed.
+End STLCTypes.
+
+Module FirstTry.
+Import STLCTypes.
+Fixpoint type_check (Gamma : context) (t : tm) : option ty :=
+  match t with
+  | tm_var x =>
+      Gamma x
+  | <{\x:T2, t1}> =>
+      match type_check (x |-> T2 ; Gamma) t1 with
+      | Some T1 => Some <{T2->T1}>
+      | _ => None
+      end
+  | <{t1 t2}> =>
+      match type_check Gamma t1, type_check Gamma t2 with
+      | Some <{T11->T12}>, Some T2 =>
+          if eqb_ty T11 T2 then Some T12 else None
+      | _,_ => None
+      end
+  | <{true}> =>
+      Some <{Bool}>
+  | <{false}> =>
+      Some <{Bool}>
+  | <{if guard then t else f}> =>
+      match type_check Gamma guard with
+      | Some <{Bool}> =>
+          match type_check Gamma t, type_check Gamma f with
+          | Some T1, Some T2 =>
+              if eqb_ty T1 T2 then Some T1 else None
+          | _,_ => None
+          end
+      | _ => None
+      end
+  end.
+End FirstTry.
+
+
+Notation " x <- e1 ;; e2" := (match e1 with
+                              | Some x => e2
+                              | None => None
+                              end)
+         (right associativity, at level 60).
+
+Notation " 'return' e " := (Some e) (at level 60).
+Notation " 'fail' " := None.
+
+Module STLCChecker.
+Import STLCTypes.
+
+Fixpoint type_check (Gamma : context) (t : tm) : option ty :=
+  match t with
+  | tm_var x =>
+      match Gamma x with
+      | Some T => return T
+      | None => fail
+      end
+  | <{\x:T2, t1}> =>
+      T1 <- type_check (x |-> T2 ; Gamma) t1 ;;
+      return <{T2->T1}>
+  | <{t1 t2}> =>
+      T1 <- type_check Gamma t1 ;;
+      T2 <- type_check Gamma t2 ;;
+      match T1 with
+      | <{T11->T12}> =>
+          if eqb_ty T11 T2 then return T12 else fail
+      | _ => fail
+      end
+  | <{true}> =>
+      return <{ Bool }>
+  | <{false}> =>
+      return <{ Bool }>
+  | <{if guard then t1 else t2}> =>
+      Tguard <- type_check Gamma guard ;;
+      T1 <- type_check Gamma t1 ;;
+      T2 <- type_check Gamma t2 ;;
+      match Tguard with
+      | <{ Bool }> =>
+          if eqb_ty T1 T2 then return T1 else fail
+      | _ => fail
+      end
+  end.
+  
+Theorem type_checking_sound : forall Gamma t T,
+  type_check Gamma t = Some T -> has_type Gamma t T.
+Proof with eauto.
+  intros Gamma t. generalize dependent Gamma.
+  induction t; intros Gamma T Htc; inversion Htc.
+  - (* var *) rename s into x. destruct (Gamma x) eqn:H.
+    rename t into T'. inversion H0. subst. eauto. solve_by_invert.
+  - (* app *)
+    remember (type_check Gamma t1) as TO1.
+    destruct TO1 as [T1|]; try solve_by_invert;
+    destruct T1 as [|T11 T12]; try solve_by_invert;
+    remember (type_check Gamma t2) as TO2;
+    destruct TO2 as [T2|]; try solve_by_invert.
+    destruct (eqb_ty T11 T2) eqn: Heqb.
+    apply eqb_ty__eq in Heqb.
+    inversion H0; subst...
+    inversion H0.
+  - (* abs *)
+    rename s into x, t into T1.
+    remember (x |-> T1 ; Gamma) as G'.
+    remember (type_check G' t0) as TO2.
+    destruct TO2; try solve_by_invert.
+    inversion H0; subst...
+  - (* tru *) eauto.
+  - (* fls *) eauto.
+  - (* test *)
+    remember (type_check Gamma t1) as TOc.
+    remember (type_check Gamma t2) as TO1.
+    remember (type_check Gamma t3) as TO2.
+    destruct TOc as [Tc|]; try solve_by_invert.
+    destruct Tc; try solve_by_invert;
+    destruct TO1 as [T1|]; try solve_by_invert;
+    destruct TO2 as [T2|]; try solve_by_invert.
+    destruct (eqb_ty T1 T2) eqn:Heqb;
+    try solve_by_invert.
+    apply eqb_ty__eq in Heqb.
+    inversion H0. subst. subst...
+Qed.
+
+Theorem type_checking_complete : forall Gamma t T,
+  has_type Gamma t T -> type_check Gamma t = Some T.
+Proof with auto.
+  intros Gamma t T Hty.
+  induction Hty; simpl.
+  - (* T_Var *) destruct (Gamma _) eqn:H0; assumption.
+  - (* T_Abs *) rewrite IHHty...
+  - (* T_App *)
+    rewrite IHHty1. rewrite IHHty2.
+    rewrite (eqb_ty_refl T2)...
+  - (* T_True *) eauto.
+  - (* T_False *) eauto.
+  - (* T_If *) rewrite IHHty1. rewrite IHHty2.
+    rewrite IHHty3. rewrite (eqb_ty_refl T1)...
+Qed.
+
+End STLCChecker.
+
+Module TypecheckerExtensions.
+Import MoreStlc.
+Import STLCExtended.
+Fixpoint eqb_ty (T1 T2 : ty) : bool :=
+  match T1,T2 with
+  | <{{Nat}}>, <{{Nat}}> =>
+      true
+  | <{{Unit}}>, <{{Unit}}> =>
+      true
+  | <{{T11 -> T12}}>, <{{T21 -> T22}}> =>
+      andb (eqb_ty T11 T21) (eqb_ty T12 T22)
+  | <{{T11 * T12}}>, <{{T21 * T22}}> =>
+      andb (eqb_ty T11 T21) (eqb_ty T12 T22)
+  | <{{T11 + T12}}>, <{{T21 + T22}}> =>
+      andb (eqb_ty T11 T21) (eqb_ty T12 T22)
+  | <{{List T11}}>, <{{List T21}}> =>
+      eqb_ty T11 T21
+  | _,_ =>
+      false
+  end.
+  
+
+Lemma eqb_ty_refl : forall T,
+  eqb_ty T T = true.
+Proof.
+  intros T.
+  induction T; simpl; auto;
+    rewrite IHT1; rewrite IHT2; reflexivity. Qed.
+
+Lemma eqb_ty__eq : forall T1 T2,
+  eqb_ty T1 T2 = true -> T1 = T2.
+Proof.
+  intros T1.
+  induction T1; intros T2 Hbeq; destruct T2; inversion Hbeq;
+    try reflexivity;
+    try (rewrite andb_true_iff in H0; inversion H0 as [Hbeq1 Hbeq2];
+         apply IHT1_1 in Hbeq1; apply IHT1_2 in Hbeq2; subst; auto);
+    try (apply IHT1 in Hbeq; subst; auto).
+ Qed.
+ 
+ 
+ 
+ 
+End STLCTypes.
